get rid of loopInv for now
we have no uses of it, and the current framework is not actually sufficient
for using loopInv (we have no infrastructure for showing the loop invariant
is preserved).  we can resurrect later if this turns out to be needed.

src/Mail2/DeliverAPI.v
@@ -121,10 +121,8 @@ End DeliverRestrictedAPI.
 
 Module DeliverTmpExistenceRule <: ProcRule DeliverAPI.
 
-  Definition loopInv (s : DeliverAPI.State) (tid : nat) := True.
-
   Definition follows_protocol (ts : @threads_state DeliverAPI.opT) :=
     forall s,
-      follows_protocol_s DeliverAPI.step DeliverRestrictedAPI.step_allow loopInv ts s.
+      follows_protocol_s DeliverAPI.step DeliverRestrictedAPI.step_allow ts s.
 
 End DeliverTmpExistenceRule.
